\documentclass[a4paper]{article}
\usepackage{amsmath,amsfonts,amsthm,amssymb}
\usepackage{geometry}
\newcommand{\cosec}{\mathrm{cosec}}

\title{Differentiation}
\date{}
\author{Gordon Chan}
\begin{document}
\maketitle
\section{Formal Definition}

\[f^\prime(x)=\lim\limits_{h\to0}\frac{f(x+h)-f(x)}h\]

\section{Example}

\[\begin{aligned}
    \ln(x)^\prime
    &=\lim\limits_{h\to0}\frac{\ln(x+h)-\ln(x)}h\\
    &=\lim\limits_{h\to0}\frac1h\ln\left(\frac{x+h}x\right)\\
    &=\lim\limits_{h\to0}\ln\left(1+\frac hx\right)^{1/h},\, t=\frac xh\\
    &=\lim\limits_{t\to\infty}\ln\left(1+\frac1t\right)^{t/x}\\
    &=\lim\limits_{t\to\infty}\ln\left(1+\frac1t\right)^{t/x}\\
    &=\ln\left(\lim\limits_{t\to\infty}\left(1+\frac1t\right)^t\right)^{\frac1x}\\
    &=\ln\left(\lim\limits_{t\to\infty}\left(1+\frac1t\right)^t\right)^{\frac1x}\\
    &=\ln(e)^{\frac1x}\\
    &=\frac1x\qed
\end{aligned}\]

\section{Product Rule}

\[(f(x)g(x))^\prime=f(x)g^\prime(x)+g(x)f^\prime(x)\]

\section{Chain Rule}

\[g(f(x))^\prime=g^\prime(f(x))f^\prime(x)\]

\section{Quotient Rule}

\[\left(\frac{f(x)}{g(x)}\right)^\prime=\frac{g(x)f^\prime(x)-f(x)g^\prime(x)}{g(x)^2}\]

\subsection{Derivation from Product Rule and Chain Rule}

\[\begin{aligned}
    \left(\frac{f(x)}{g(x)}\right)^\prime
    &=\left(f(x)\frac1{g(x)}\right)^\prime\\
    &=f(x)\left(\frac1{g(x)}\right)^\prime+\frac1{g(x)}f^\prime(x)\\
    &=f(x)\left(-\frac1{g(x)^2}g^\prime(x)\right)+\frac{f^\prime(x)}{g(x)}\\
    &=-\frac{f(x)g^\prime(x)}{g(x)^2}+\frac{g(x)f^\prime(x)}{g(x)^2}\\
    &=\frac{g(x)f^\prime(x)-f(x)g^\prime(x)}{g(x)^2}\qed
\end{aligned}\]

\section{Table of Derivatives}

\[\def\arraystretch{2}
\begin{array}[t]{|c|c|}
    \hline
    f(x)&f^\prime(x)\\
    \hline
    \sin^{-1}(x)&\displaystyle\frac1{\sqrt{1-x^2}}\\
    \cos^{-1}(x)&\displaystyle-\frac1{\sqrt{1-x^2}}\\
    \tan^{-1}(x)&\displaystyle\frac1{1+x^2}\\
    \cosec^{-1}(x)&\displaystyle-\cosec(x)\cot(x)\\
    \sec^{-1}(x)&\displaystyle\sec(x)\tan(x)\\
    \hline
\end{array}\]

\end{document}
