\documentclass[a4paper]{article}

\usepackage{amsmath,amsfonts,amsthm,amssymb}
\usepackage[margin=1in]{geometry}
\author{\(\mathbb{GONDRO}\)}
\title{Euclidean Algorithm}

\begin{document}
\maketitle
\section{Proof}
Suppose \(a\) and \(b\) are positive integers.
By \emph{Euclidean division lemma},
\[(\forall a,b\in\mathbb Z)(b\ne0)(\exists b,r\in\mathbb Z)(0\leqslant r<|b|)(a=bq+r)\]
Thus,
\[(\exists b,r\in\mathbb Z)(0\leqslant r<|b|)(a=bq+r\land r=a-bq)\]
Let \(h=\gcd(a,b)\) and \(g=\gcd(b,r)\).
\[\begin{aligned}
    g&=\gcd(b,r)\\
    \implies g\mid b&\land g\mid r\\
    \implies (\exists m,n\in\mathbb Z)(gm=b&\land gn=r)\\
    \implies gqm=bq&\land gn=r\\
    \implies gqm+gn&=bq+r\\
    \implies g(qm+n)&=bq+r\\
    \implies g&\mid bq+r\\
    \implies g&\mid a
\end{aligned}\]
\[g\mid a\land g\mid b\implies g\mid h\implies g\leqslant h\]

\[\begin{aligned}
    h&=\gcd(a,b)\\
    \implies h\mid a&\land h\mid b\\
    \implies (\exists m,n\in\mathbb Z)(hk=a&\land hj=b)\\
    \implies hk=a&\land hqj=qb\\
    \implies hk-hqj&=a-qb\\
    \implies h(k-qj)&=a-qb\\
    \implies h&\mid a-qb\\
    \implies h&\mid r
\end{aligned}\]
\[h\mid b\land h\mid r\implies h\mid g\implies h\leqslant g\]

\[g\leqslant h\land h\leqslant g\implies h=g\]

\[\therefore a=bq+r\implies\gcd(a,b)=\gcd(b,r)\qed\]

\section{Example Application}
Compute \(\gcd(2322,654)\).

\[\begin{array}{c|c}
\begin{aligned}
    &\gcd(2322,654)\\
    &=\gcd(654,360)\\
    &=\gcd(360,294)\\
    &=\gcd(294,66)\\
    &=\gcd(66,30)\\
    &=\gcd(30,6)\\
    &=\boxed6
\end{aligned}
    &
\begin{aligned}
    2322&=654\cdot3+360\\
    654&=360\cdot1+294\\
    360&=294\cdot1+66\\
    294&=66\cdot4+30\\
    66&=30\cdot2+6\\
    30&=6\cdot5+0
\end{aligned}
\end{array}\]
Solve for all integer solutions of \(2322x+654y=\gcd(2322,654)\).\\
By rearranging the equations above,
\[\begin{aligned}
    360&=2322-654\cdot3\\
    294&=654-360\cdot1\\
    66&=360-294\cdot1\\
    30&=294-66\cdot4\\
    6&=66-30\cdot2
\end{aligned}\]

\[\begin{aligned}
    \gcd(2322,654)&=6\\
    &=66-30\cdot2\\
    &=66-(294-66\cdot4)\cdot2\\
    &=66-294\cdot2+66\cdot8\\
    &=66\cdot9-294\cdot2\\
    &=(360-294\cdot1)\cdot9-294\cdot2\\
    &=360\cdot9-294\cdot9-294\cdot2\\
    &=360\cdot9-294\cdot11\\
    &=360\cdot9-(654-360\cdot1)\cdot11\\
    &=360\cdot9-654\cdot11+360\cdot11\\
    &=360\cdot20-654\cdot11\\
    &=(2322-654\cdot3)\cdot20-654\cdot11\\
    &=2322\cdot20-654\cdot60-654\cdot11\\
    &=2322\cdot20-654\cdot71
\end{aligned}\]

\[2322(20)+654(-71)=\gcd(2322,654)\]
Now solve for the homogeneous case: \(2322x+654y=0\).\\
Notice that \(2322=6\cdot387\) and \(654=6\cdot109\).\\
Hence, the lowest common multiple of 2322 and 654 is \(6\cdot109\cdot387\).\\
Thus, \(2322(109t)+654(-387t)=0\)

\[\therefore2322(20+109t)+654(-71-387t)=\gcd(2322,654)\]

\[\begin{cases}
    x=\boxed{20+109t}\\
    y=\boxed{-71-387t}
\end{cases}
,\,t\in\mathbb Z\]
\end{document}
