\documentclass[a4paper,12pt]{article}
\usepackage{amsmath,amsfonts,amsthm,amssymb}
\usepackage{physics}
\usepackage[margin=1in]{geometry}
\title{Solution for The Pure Mathematics Portion of\\
GCE `A' Levels Further Mathematics Paper 2}
\author{Gordon Chan}

\begin{document}
\maketitle

\section*1
\subsection*{(i)}
Let \(\vb A=\bmqty{1&-1&2&-1&5\\1&3&-2&1&-1\\1&0&1&3&0\\0&1&-1&1&2}\) and \(\vb x=\bmqty{x_1\\x_2\\x_3\\x_4\\x_5}\).
\[\begin{aligned}
    \vb A=\bmqty{1&-1&2&-1&5\\1&3&-2&1&-1\\1&0&1&3&0\\0&1&-1&1&2}
     &\to\bmqty{1&-1&2&-1&5\\0&4&-4&2&-6\\0&1&-1&4&-5\\0&1&-1&1&2}\\
      \to\bmqty{1&-1&2&-1&5\\0&1&-1&\frac12&-\frac32\\0&1&-1&4&-5\\0&1&-1&1&2}
     &\to\bmqty{1&0&1&-\frac12&\frac72\\0&1&-1&\frac12&-\frac32\\0&0&0&\frac72&-\frac72\\0&0&0&\frac12&\frac72}\\
      \to\bmqty{1&0&1&0&3\\0&1&-1&0&-1\\0&0&0&\frac72&-\frac72\\0&0&0&0&4}
     &\to\bmqty{1&0&1&0&3\\0&1&-1&0&-1\\0&0&0&1&-1\\0&0&0&0&1}\\
      \to\bmqty{1&0&1&0&0\\0&1&-1&0&0\\0&0&0&1&0\\0&0&0&0&1}&=\text{rref}(\vb A)
\end{aligned}\]
\[\vb A\vb x=\vb0
\implies
\text{rref}(\vb A)\vb x=\vb0
\implies
\begin{cases}
    x_1+x_3=0\\
    x_2-x_3=0\\
    x_4=0\\
    x_5=0
\end{cases}
\implies
\begin{cases}
    x_1=-x_3\\
    x_2=x_3\\
    x_4=0\\
    x_5=0
\end{cases}\]
\[\vb x=\bmqty{x_1\\x_2\\x_3\\x_4\\x_5}
    =\bmqty{-x_3\\x_3\\x_3\\0\\0}
=x_3\bmqty{-1\\1\\1\\0\\0},
\,x_3\in\mathbb R\]
\[S=\ker(\vb A)\implies 
B_S=B_{\ker(\vb A)}
=\boxed{\Bqty{\bmqty{-1\\1\\1\\0\\0}}}\]
\subsection*{(ii)}
\[\dim(S)=\dim(\ker\vb A)=\boxed1\]

\section*2
\subsection*{(i)}
\[\begin{aligned}
    z^7&=1\\
    z^7&\equiv e^{i(2\pi m)},\,m\in\{0,\pm1,\pm2,\pm3\}\\
z&\in\Bqty{1,e^{i\pqty{\pm\frac{2\pi}7}},e^{i\pqty{\pm\frac{4\pi}7}},e^{i\pqty{\pm\frac{6\pi}7}}}
\end{aligned}\]
\[\begin{aligned}
    z^7-1&=(z-1)\prod_{n=1}^3\pqty{z-e^{i\pqty{\frac{2n\pi}7}}}\pqty{z-e^{i\pqty{-\frac{2n\pi}7}}}\\
    \frac{z^7-1}{z-1}&=\prod_{n=1}^3\pqty{z^2-\pqty{2\cos\frac{2n\pi}7}z+e^{i\pqty{0}}}\\
    \sum_{n=0}^6z^n&=\boxed{\pqty{z^2-\pqty{2\cos\frac{2\pi}7}z+1}\pqty{z^2-\pqty{2\cos\frac{4\pi}7}z+1}\pqty{z^2-\pqty{2\cos\frac{6\pi}7}z+1}}
\end{aligned}\]
\subsection*{(ii)}
\[\begin{aligned}
    &\cos\pqty{\frac17\pi}-\cos\pqty{\frac27\pi}+\cos\pqty{\frac37\pi}\\
    &=\cos\pqty{\frac17\pi}-2\cos^2\pqty{\frac17\pi}+1+4\cos^3\pqty{\frac17\pi}-3\cos\pqty{\frac17\pi}\\
    &=1-\pqty{}
\end{aligned}\]
\subsection*{(iii)}
\[\begin{aligned}
    &\cos\pqty{\frac17\pi}\cos\pqty{\frac27\pi}\cos\pqty{\frac37\pi}\\
    &=\frac{2\sin\pqty{\frac17\pi}}{2\sin\pqty{\frac17\pi}}\cos\pqty{\frac17\pi}\cos\pqty{\frac27\pi}\cos\pqty{\frac37\pi}\\
\end{aligned}\]

\section*3
\subsection*{(i)}
\subsubsection*{(a)}
\[T(\vb v)=\vb A\vb v=\bmqty{-1&7\\2&-6}\bmqty{6\\1}=\bmqty{1\\6}\]
\end{document}
