\documentclass[a4paper]{article}
\usepackage{amsmath,amsfonts,amsthm,amssymb}
\usepackage{geometry}
\usepackage{graphicx}
\usepackage{physics}
\usepackage{centernot}

\begin{document}
\section*1
\subsection*{(a)}
\[((\neg s\land l)\lor s)\centernot\implies(s\implies\neg l)\]
\subsection*{(b)}

\section*2
\[(a\mid b\iff b=na)\land(b\mid c\iff c=mb)\]
    \[c=nb=n(ma)=(nm)a\iff c\mid a\qed\]

\section*3
\[x\in\mathbb Z\]
Suppose \(2\mid x^2-1\).
\[\begin{aligned}
    2&\mid x^2-1\\
    x^2-1&=2a\\
    (x-1)(x+1)&=2a
\end{aligned}\]
For \((x-1)(x+1)\) to be even, \((x-1)\lor(x+1)\) must be even. Suppose \(x-1=2n\).
\[\begin{aligned}
    x-1&=2n\\
    x+1&=2n+2\\
    x+1&=2(n+1)\\
    (x-1)(x+1)&=(2n)(2(n+1))\\
    x^2-1&=4\left(n^2+1\right)
\end{aligned}\]
WLOG, same thing happens when \((x+1)\) is even or \((x-1)\land(x+1)\) are even.\qed{}

\section*4
\subsection*{(i)}
Case 1: \(a=k,\,k\in\mathbb R^+\).
\[a^2=aa=kk=k^2>0\]
Case 2: \(a=-k,\,k\in\mathbb R^+\).
\[a^2=aa=(-k)(-k)=k^2>0\]
Case 3: \(a=0\).
\[a^2=(0)(0)=0\]
Thus, \(\forall a\in\mathbb R\), \(a^2\geqslant0\).\qed{}
\subsection*{(ii)}
\[\begin{aligned}
    {(a-b)}^2&\geqslant0\\
    a^2-2ab+b^2&\geqslant0\\
    -2ab&\geqslant-\pqty{a^2+b^2}\\
    ab&\leqslant\frac12\pqty{a^2+b^2}\qed
\end{aligned}\]
\subsection*{(iii)}
\[\begin{aligned}
    {(ca-c^{-1}b)}^2&\geqslant0\\
    c^2a^2-2ab+c^{-2}b^2&\geqslant0\\
    -2ab&\geqslant-\pqty{c^2a^2+c^{-2}b^2}\\
    ab&\leqslant\frac12\pqty{c^2a^2+c^{-2}b^2}\qed
\end{aligned}\]

\section*5
\subsection*{(i)}
\[\begin{aligned}
    {(\alpha y-\beta x)}^2&\geqslant0\\
    \alpha^2y^2-2\alpha\beta xy+\beta^2x^2&\geqslant0\\
    \frac{\alpha^2}{x^2}+\frac{\beta^2}{y^2}&\geqslant\frac{2\alpha\beta}{xy}
\end{aligned}\]
\end{document}
