\documentclass[a4paper]{article}
\usepackage{amsmath,amsfonts,amsthm,amssymb}
\usepackage{geometry}
\usepackage{physics}

\begin{document}
\section*4
Let \(P(n):\sum\limits_{r=1}^n\sin(2rx)\sin x=\sin(nx)\sin(n+1)x\).
\[n=1\implies\sum\limits_{r=1}^1\sin(2rx)\sin x=\sin(2x)\sin x=\sin(1x)\sin(1+1)x
\implies P(1)\to\top\]
Assume \(\left(\exists k\in\mathbb Z^+\right)P(n)\to\top\implies\sum\limits_{r=1}^k\sin(2rx)\sin x=\sin(kx)\sin(k+1)x\).
\[\begin{aligned}
    n=k+1\implies&\phantom{=}\sum\limits_{r=1}^n\sin(2rx)\sin x\\
         &=\sum\limits_{r=1}^{k+1}\sin(2rx)\sin x\\
         &=\sum\limits_{r=1}^{k}\sin(2rx)\sin x+\sin(2(k+1)x)\sin x\\
         &=\sin(kx)\sin(k+1)x+\sin(2(k+1)x)\sin x\\
         &=\sin(kx)\sin(kx+x)+\sin(2kx+2x)\sin x\\
         &=-\frac12\left(-2\sin\frac12(2kx)\sin\frac12(2kx+2x)-2\sin\frac12(4kx+4x)\sin\frac12(2x)\right)\\
         &=-\frac12\left(\cos(2kx+x)-\cos x+\cos(2kx+3x)-\cos(2kx+x)\right)\\
         &=-\frac12\left(\cos(2kx+3x)-\cos x\right)\\
         &=-\frac12\left(-2\sin\frac12(2kx+4x)\sin\frac12(2kx+2x)\right)\\
         &=\sin(kx+2x)\sin(kx+x)\\
         &=\sin(k+1)x\sin((k+1)+1)x\\
         &=\sin(nx)\sin(n+1)x\implies P(n+1)\to\top
\end{aligned}\]
\[((P(1)\to\top)\land(P(k)\to\top\implies P(k+1)\to\top))\implies\left(\forall n\in\mathbb Z^+\right)P(n)\to\top\]
\[\therefore\sum\limits_{r=1}^n\sin(2rx)\sin x=\sin(nx)\sin(n+1)x,\,\forall n\in\mathbb Z^+\qed\]
\[\begin{aligned}
    \int_{\frac\pi4}^{\frac\pi2}\frac{\sin3x\sin4x}{\sin x}\dd{x}
    &=\int_{\frac\pi4}^{\frac\pi2}\frac{\sin3x\sin(3+1)x}{\sin x}\dd{x}\\
    &=\int_{\frac\pi4}^{\frac\pi2}\frac{\sum\limits_{r=1}^3\sin(2rx)\sin x}{\sin x}\dd{x}\\
    &=\int_{\frac\pi4}^{\frac\pi2}\frac{\sin(2x)\sin x+\sin(4x)\sin x+\sin(6x)\sin x}{\sin x}\dd{x}\\
    &=\int_{\frac\pi4}^{\frac\pi2}\left(\sin(2x)+\sin(4x)+\sin(6x)\right)\dd{x}\\
    &=\eval{\pqty{-\frac12\cos2x-\frac14\cos4x-\frac16\cos6x}}_{\frac\pi4}^{\frac\pi2}\\
    &=-\frac12(-1)-\frac14(0)-\frac16(-1)\\
    &=\boxed{\frac23}
\end{aligned}\]

\section*5
Let \(P(n):7\mid10^{3n}+13^{n+1}\).
\[n=1\implies10^{3n}+13^{n+1}=10^3+13^2=1169=7(169)\implies P(1)\to\top\]
Assume \(\left(\exists k\in\mathbb Z^+\right)P(k)\to\top\implies7\mid10^{3k}+13^{k+1}\).
\[\begin{aligned}
    10^{3k}+13^{k+1}&=7m,\,m\in\mathbb Z\\
    13^{k+1}&=7m-10^{3k}
\end{aligned}\]
\[\begin{aligned}
    n=k+1\implies10^{3n}+13^{n+1}&=10^{3(k+1)}+13^{(k+1)+1}\\
                    &=10^{3k+3}+13^{k+2}\\
                    &=1000\cdot10^{3k}+13\cdot13^{k+1}\\
                    &=1000\left(10^{3k}\right)+13\left(7m-10^{3k}\right)\\
                    &=1000\left(10^{3k}\right)+13(7m)-13\left(10^{3k}\right)\\
                    &=987\left(10^{3k}\right)+7(13m)\\
                    &=7\cdot141\left(10^{3k}\right)+7(13m)\\
                    &=7\left(141\left(10^{3k}\right)+13m\right)\\
                    &=7M,\,M\in\mathbb Z\implies P(k+1)\to\top\\
\end{aligned}\]
\[((P(1)\to\top)\land(P(k)\to\top\implies P(k+1)\to\top))\implies\left(\forall n\in\mathbb Z^+\right)P(n)\to\top\]
\[\therefore7\mid10^{3n}+13^{n+1},\,\forall n\in\mathbb Z^+\qed\]
\end{document}
