\documentclass[a4paper]{article}
\usepackage{amsmath,amsfonts,amsthm,amssymb}

\begin{document}

\[y-\bar y=b(x-\bar x)\iff y=(\bar y-b\bar x)+bx\equiv y=a+bx\]

\[\implies a=\bar y-b\bar x\]

\[\begin{aligned}
	v_i&=y_i-(a+bx_i)\\
	&=y_i-(\bar y-b\bar x+bx_i)\\
	&=y_i-\bar y+b(\bar x-x_i)\\
	\sum v_i^2&=\sum(y_i-\bar y+b(\bar x-x_i))^2\\
	\left(\sum v_i^2\right)^\prime&=\sum2(y_i-\bar y+b(\bar x-x_i))(\bar x-x_i)\\
\end{aligned}\]

\[\begin{aligned}
	\left(\sum v_i^2\right)^\prime&=0\\
	\sum2(y_i-\bar y+b(\bar x-x_i))(\bar x-x_i)&=0\\
	\sum(y_i-\bar y)(\bar x-x_i)+b\sum (\bar x-x_i)^2&=0\\
	b\sum (x_i-\bar x)^2&=\sum(y_i-\bar y)(x_i-\bar x)\\
	b&=\boxed{\frac{\sum(y_i-\bar y)(x_i-\bar x)}{\sum (x_i-\bar x)^2}}\\
\end{aligned}\]
\end{document}
