\documentclass[a4paper,12pt]{article}
\usepackage{amsmath}
\usepackage{amsfonts}
\usepackage{amsthm}
\usepackage{amssymb}
\usepackage{setspace}
\title{Algebaric Simplification}
\date{}
\author{}
\doublespacing{}
\begin{document}
\maketitle

\section{Substitution}
In algebra, 
the operation of substitution is applied in contexts involving variables;
the operation consists of replacing occurrences of some symbol by given values.
\subsection{Example}
It is given that \(f(x,y)=\displaystyle\frac x{2x+y}-\frac yx\), compute \(f(5,-2)\).
\[\begin{aligned}
    f(5,-2)&=\frac5{2(5)+(-2)}-\frac5{-2}\\
           &=\frac5{10-2}-\frac52\\
           &=\frac58+\frac{20}8\\
           &=\boxed{\frac{25}8}
\end{aligned}\]

\newpage

\section{Multiplication and Division}
Simplify each of the following.
\[3a\times5a\]
\[27a\div9b\times3c\]

\section{Expansion}
Expand and Simplify \(2(a+b)-3(2a-b)\).
\[\begin{aligned}
    2(a+b)-3(2a-b)&=2a+2b-(6a-3b)\\
                  &=2a+2b-6a+3b\\
                  &=2a-6a+2b+3b\\
                  &=\boxed{-4a+5b}
\end{aligned}\]

\section{Fraction}
Express \(\displaystyle\frac{x-2}4+\frac{2x-2}6\) as a single fraction in its simplest form.
\[\begin{aligned}
    \frac{x-2}4+\frac{2x-2}6&=\frac{3(x-2)}{12}+\frac{2(2x-2)}{12}\\
                            &=\frac{3x-6+4x-4}{12}\\
                            &=\boxed{\frac{7x-10}{12}}
\end{aligned}\]

\section{Factorisation}
Identify the HCF of each of the following and factorise the expressions.
\[12xy-36yz\]
\[4x-8x^2\]
\end{document}
