\documentclass[12pt,a4paper]{article}
\usepackage{amsmath}
\usepackage{amsfonts}
\usepackage{amsthm}
\usepackage{amsfonts}
\begin{document}
\[\begin{aligned}
\sum\limits_{n}e^{i(x+\varphi_n)}&=\sum\limits_{n}(\cos(x+\varphi_n)+i\sin(x+\varphi_n))\\
&=\sum\limits_{n}\cos(x+\varphi_n)+\sum\limits_{n}i\sin(x+\varphi_n)\\
&=\sum\limits_{n}\cos(x+\varphi_n)+i\sum\limits_{n}\sin(x+\varphi_n)\\
\end{aligned}\]

\[\begin{aligned}
\sum\limits_{n}e^{i(x+\varphi_n)}&=\sum\limits_{n}e^{ix+i\varphi_n}\\
&=\sum\limits_{n}e^{ix}e^{i\varphi_n}\\
&=e^{ix}\sum\limits_{n}e^{i\varphi_n}\\
&=e^{ix}\sum\limits_{n}(\cos(\varphi_n)+i\sin(\varphi_n))\\
&=e^{ix}\left(\sum\limits_{n}\cos(\varphi_n)+\sum\limits_{n}i\sin(\varphi_n)\right)\\
&=e^{ix}\left(\sum\limits_{n}\cos(\varphi_n)+i\sum\limits_{n}\sin(\varphi_n)\right)\\
&=e^{ix}(A+iB)\\
&=e^{ix}\sqrt{A^2+B^2}e^{i\arg(A+iB)}\\
&=\sqrt{A^2+B^2}e^{ix+i\arg(A+iB)}\\
&=\sqrt{A^2+B^2}e^{i(x+\arg(A+iB))}\\
&=\sqrt{A^2+B^2}(\cos(x+\arg(A+iB))+i\sin(x+\arg(A+iB)))\\
&=\sqrt{A^2+B^2}\cos(x+\arg(A+iB))+i\sqrt{A^2+B^2}\sin(x+\arg(A+iB))
\end{aligned}\]

\[\boxed{
\begin{cases}
\sum\limits_{n}\sin(x+\varphi_n)=\sqrt{A^2+B^2}\sin(x+\arg(A+iB))\\
\sum\limits_{n}\cos(x+\varphi_n)=\sqrt{A^2+B^2}\cos(x+\arg(A+iB))\\
A=\sum\limits_{n}\cos(\varphi_n)\\
B=\sum\limits_{n}\sin(\varphi_n)
\end{cases}}\] 
\newpage
Example:

\[\begin{aligned}
&\phantom{=}\sin(2\pi(t+e))+\sin(2\pi t+69)+\sin(2\pi t+42^\circ)\\
&=\sin(2\pi t+2\pi e)+\sin(2\pi t+69)+\sin(2\pi t+42^\circ)\\
&=\sqrt{A^2+B^2}\sin(2\pi t+\arg(A+iB))
\end{aligned}\]
\[\begin{cases}
A=\cos(2\pi e)+\cos(69)+\cos(42^\circ)\approx1.53856064504\\
B=\sin(2\pi e)+\sin(69)+\sin(42^\circ)\approx-0.425861365902
\end{cases}\]
\[\sqrt{A^2+B^2}\approx1.59641058674\]
\[\arg(A+iB)=\tan^{-1}\left(\frac BA\right)\approx-15.4716657207^\circ\]
\[\sin(2\pi(t+e))+\sin(2\pi t+69)+\sin(2\pi t+42^\circ)\approx\boxed{1.60\sin(2\pi t-15.5^\circ)}\]
\end{document}
