\documentclass{article}
\usepackage{amsmath}
\usepackage{amsthm}
\usepackage{amssymb}
\usepackage{amsfonts}
\begin{document}
\[\begin{aligned}
S&=\sum_{n=a}^{b}r^n\\
S&=r^a+r^{a+1}+r^{a+2}+\cdots+r^{b-2}+r^{b-1}+r^b\\
rS&=r^{a+1}+r^{a+2}+\cdots+r^{b-2}+r^{b-1}+r^b+r^{b+1}\\
rS&=r^a+r^{a+1}+r^{a+2}+\cdots+r^{b-2}+r^{b-1}+r^b+r^{b+1}-r^a\\
rS&=S+r^{b+1}-r^a\\
rS-S&=r^{b+1}-r^a\\
S(r-1)&=r^{b+1}-r^a\\
S&=\frac{r^{b+1}-r^a}{r-1}
\end{aligned}\]
\\
\[\therefore\boxed{\sum_{n=a}^{b}r^n=\frac{r^{b+1}-r^a}{r^{0+1}-r^0}}\]
Henlo
\end{document}
