\documentclass[a4paper]{article}
\usepackage{amsmath,amsfonts,amsthm,amssymb}

\begin{document}

\[\begin{aligned}
    E(aX+bY)&=E(aX)+E(bY)\\
    &=aE(X)+bE(Y)
\end{aligned}\]

\[\begin{aligned}
    E\left(\frac{(n_1-1)s_1^2+(n_2-1)s_2^2}{n_1+n_2-2}\right)
    &=
\end{aligned}\]

\[\sum_{i=1}^\nu Z_i^2\sim\chi^2(\nu)\]
\[(\mu,\sigma^2)=(\nu,2\nu)\]
\[f(x)=
\begin{cases}
    \displaystyle\frac{x^{\frac\nu2-1}e^{-\frac x2}}{2^{\frac\nu2}\Gamma\left(\frac\nu2\right)},\,x\geqslant0\\
    0,\,\text{otherwise}
\end{cases}\]
\end{document}
