\documentclass[a4paper]{article}
\usepackage{amsmath,amsfonts,amsthm,amssymb}
\usepackage{graphicx}
\usepackage{concmath}
\usepackage[T1]{fontenc}
\makeatletter
\renewcommand*\env@matrix[1][*\c@MaxMatrixCols c]{%
  \hskip -\arraycolsep
  \let\@ifnextchar\new@ifnextchar
  \array{#1}}
\makeatother
\begin{document}
\def\arraystretch{1.25}
9.
(i)
\[{\bf A}=
\begin{bmatrix}
1&-2&1&3\\
2&1&5&-7\\
4&-3&7&^-1\\
3&14&15&-43
\end{bmatrix}
\overset{\text{rref}}{\longrightarrow}
\begin{bmatrix}
	1&0&\frac{11}5&-\frac{11}5\\
0&1&\frac35&-\frac{13}5\\
0&0&0&0\\
0&0&0&0
\end{bmatrix}\]
\[{\bf K}=\ker({\bf A})=
	\left\{\begin{bmatrix}x_1\\x_2\\x_3\\x_4\end{bmatrix}:
\begin{bmatrix}
	1&0&\frac{11}5&-\frac{11}5\\
0&1&\frac35&-\frac{13}5\\
0&0&0&0\\
0&0&0&0
\end{bmatrix}
\begin{bmatrix}x_1\\x_2\\x_3\\x_4\end{bmatrix}
=\begin{bmatrix}0\\0\\0\\0\end{bmatrix}
\right\}\]
\[\implies\begin{cases}
	x_4=\mu\\
	x_3=\lambda\\
	x_2=-\frac35\lambda+\frac{13}5\mu\\
	x_1=-\frac{11}5\lambda+\frac{11}5\mu
\end{cases},\,\lambda,\mu\in\mathbb R\]
\[{\bf K}=
	\left\{\lambda\begin{bmatrix}-11\\-3\\5\\0\end{bmatrix}+\mu\begin{bmatrix}11\\13\\0\\5\end{bmatrix},\,\lambda,\mu\in\mathbb R\right\}
\]
When \(\lambda=\mu=0\), \(\lambda\begin{bmatrix}-11\\-3\\5\\0\end{bmatrix}+\mu\begin{bmatrix}11\\13\\0\\5\end{bmatrix}={\bf 0}\in{\bf K}\). 

Let \({\bf k}_{i,j}=\lambda_i\begin{bmatrix}-11\\-3\\5\\0\end{bmatrix}+\mu_j\begin{bmatrix}11\\13\\0\\5\end{bmatrix}\in{\bf K}\).
\[\begin{aligned}
	\alpha{\bf k}_{1,1}+\beta{\bf k}_{2,2}&=\alpha\left(\lambda_1\begin{bmatrix}-11\\-3\\5\\0\end{bmatrix}+\mu_1\begin{bmatrix}11\\13\\0\\5\end{bmatrix}\right)+\beta\left(\lambda_2\begin{bmatrix}-11\\-3\\5\\0\end{bmatrix}+\mu_2\begin{bmatrix}11\\13\\0\\5\end{bmatrix}\right)\\
&=\alpha\lambda_1\begin{bmatrix}-11\\-3\\5\\0\end{bmatrix}+\alpha\mu_1\begin{bmatrix}11\\13\\0\\5\end{bmatrix}+\beta\lambda_2\begin{bmatrix}-11\\-3\\5\\0\end{bmatrix}+\beta\mu_2\begin{bmatrix}11\\13\\0\\5\end{bmatrix}\\
&=(\alpha\lambda_1+\beta\lambda_2)\begin{bmatrix}-11\\-3\\5\\0\end{bmatrix}+(\alpha\mu_1+\beta\mu_2)\begin{bmatrix}11\\13\\0\\5\end{bmatrix}\in{\bf K}
\end{aligned}\]
Therefore, \(\bf K\) is a vector space.\qed
\[\dim({\bf K})=\boxed2\]

(ii)
\[[{\bf A}|{\bf b}]=
	\begin{bmatrix}[cccc|c]
		1&-2&1&3&3\\
		2&1&5&-7&1\\
		4&-3&7&-1&7\\
		3&14&15&-43&-11
	\end{bmatrix}
\overset{\text{rref}}{\longrightarrow}
	\begin{bmatrix}[cccc|c]
		1&0&\frac{11}5&-\frac{11}5&1\\
		0&1&\frac35&-\frac{13}5&-1\\
		0&0&0&0&0\\
		0&0&0&0&0
	\end{bmatrix}\]
\[S=
	\left\{\begin{bmatrix}x_1\\x_2\\x_3\\x_4\end{bmatrix}:
\begin{bmatrix}
	1&0&\frac{11}5&-\frac{11}5\\
0&1&\frac35&-\frac{13}5\\
0&0&0&0\\
0&0&0&0
\end{bmatrix}
\begin{bmatrix}x_1\\x_2\\x_3\\x_4\end{bmatrix}
=\begin{bmatrix}1\\-1\\0\\0\end{bmatrix}
\right\}\]
\[\implies\begin{cases}
	x_4=\mu\\
	x_3=\lambda\\
	x_2=-1-\frac35\lambda+\frac{13}5\mu\\
	x_1=1-\frac{11}5\lambda+\frac{11}5\mu
\end{cases},\,\lambda,\mu\in\mathbb R\]
\[S=\left\{\begin{bmatrix}1\\-1\\0\\0\end{bmatrix}+
\lambda\begin{bmatrix}-11\\-3\\5\\0\end{bmatrix}+\mu\begin{bmatrix}11\\13\\0\\5\end{bmatrix},\,\lambda,\mu\in\mathbb R\right\}
\]
Suppose \((\exists s_p\in S)(s_p={\bf 0})\).
\[\begin{bmatrix}1\\-1\\0\\0\end{bmatrix}+
\lambda_p\begin{bmatrix}-11\\-3\\5\\0\end{bmatrix}+\mu_p\begin{bmatrix}11\\13\\0\\5\end{bmatrix}=\begin{bmatrix}0\\0\\0\\0\end{bmatrix}\]
\[
	\implies\begin{cases}
	0+5\lambda_p+0\mu_p=0\\
	0+0\lambda_p+5\mu_p=0\\
	1-11\lambda_p+11\mu_p=0
\end{cases}
	\implies\begin{cases}
		\lambda_p=0\\
		\mu_p=0\\
		1=0
\end{cases}
\implies\impliedby
\]
\[\implies{\bf0}\not\in S\]
Therefore, \(S\) is not a vector space.
\end{document}
